theories/Terms.v
@@ -1,0 +1,143 @@
+(** * Preliminaries FOL*  *)
+
+From Equations Require Import Equations.
+Require Import Equations.Prop.DepElim.
+
+Ltac capply H := eapply H; try eassumption.
+
+Ltac resolve_existT :=
+  match goal with
+     | [ H2 : existT _ _ _ = existT _ _ _ |- _ ] => rewrite (Eqdep.EqdepTheory.inj_pair2 _ _ _ _ _ H2) in *
+  | _ => idtac
+  end.
+
+Ltac inv H :=
+  inversion H; subst; repeat (progress resolve_existT).
+
+
+
+(** ** Syntax of FOL* **)
+
+From Undecidability.FOLC Require Export unscoped.
+
+Notation vector := Vector.t.
+Import Vector.
+Arguments nil {A}.
+Arguments cons {A} _ {n}.
+Derive Signature for vector.
+
+Class Signature := B_S { Funcs : Type; fun_ar : Funcs -> nat ;
+              Preds : Type; pred_ar : Preds -> nat }.
+
+
+Section fix_sig.
+
+Context {Sigma : Signature}.
+
+Inductive term  : Type :=
+  | var_term : (fin)  -> term
+  | Func : forall (f : Funcs), Vector.t term (fun_ar f) -> term .
+
+Definition congr_Func { f : Funcs }  { s0 : Vector.t term (fun_ar f) } { t0 : Vector.t term (fun_ar f)} (H1 : s0 = t0) : Func  f s0 = Func  f t0 :=
+  (eq_trans) (eq_refl) ((ap) (fun x => Func  f x) H1).
+
+Fixpoint subst_term   (sigmaterm : (fin)  -> term ) (s : term ) : _ :=
+    match s with
+    | var_term  s => sigmaterm s
+    | Func  f s0 => Func  f (Vector.map (subst_term sigmaterm) s0)
+    end.
+
+Definition up_term_term   (sigma : (fin)  -> term ) : _ :=
+  (scons) ((var_term ) (var_zero)) ((funcomp) (subst_term ((funcomp) (var_term ) (shift))) sigma).
+
+
+Definition upId_term_term  (sigma : (fin)  -> term ) (Eq : forall x, sigma x = (var_term ) x) : forall x, (up_term_term sigma) x = (var_term ) x :=
+  fun n => match n with
+  | S fin_n => (ap) (subst_term ((funcomp) (var_term ) (shift))) (Eq fin_n)
+  | 0 => eq_refl
+  end.
+
+
+Fixpoint idSubst_term  (sigmaterm : (fin)  -> term ) (Eqterm : forall x, sigmaterm x = (var_term ) x) (s : term ) : subst_term sigmaterm s = s :=
+    match s with
+    | var_term  s => Eqterm s
+    | Func  f s0 => congr_Func ((vec_id (idSubst_term sigmaterm Eqterm)) s0)
+    end.
+
+Definition upExt_term_term   (sigma : (fin)  -> term ) (tau : (fin)  -> term ) (Eq : forall x, sigma x = tau x) : forall x, (up_term_term sigma) x = (up_term_term tau) x :=
+  fun n => match n with
+  | S fin_n => (ap) (subst_term ((funcomp) (var_term) (shift))) (Eq fin_n)
+  | 0 => eq_refl
+  end.
+
+
+Fixpoint ext_term   (sigmaterm : (fin)  -> term ) (tauterm : (fin)  -> term ) (Eqterm : forall x, sigmaterm x = tauterm x) (s : term ) : subst_term sigmaterm s = subst_term tauterm s :=
+    match s with
+    | var_term  s => Eqterm s
+    | Func  f s0 => congr_Func ((vec_ext (ext_term sigmaterm tauterm Eqterm)) s0)
+    end.
+
+Fixpoint compSubstSubst_term    (sigmaterm : (fin)  -> term ) (tauterm : (fin)  -> term ) (thetaterm : (fin)  -> term ) (Eqterm : forall x, ((funcomp) (subst_term tauterm) sigmaterm) x = thetaterm x) (s : term ) : subst_term tauterm (subst_term sigmaterm s) = subst_term thetaterm s :=
+    match s with
+    | var_term  s => Eqterm s
+    | Func  f s0 => congr_Func ((vec_comp (compSubstSubst_term sigmaterm tauterm thetaterm Eqterm)) s0)
+    end.
+
+Definition up_subst_subst_term_term    (sigma : (fin)  -> term ) (tauterm : (fin)  -> term ) (theta : (fin)  -> term ) (Eq : forall x, ((funcomp) (subst_term tauterm) sigma) x = theta x) : forall x, ((funcomp) (subst_term (up_term_term tauterm)) (up_term_term sigma)) x = (up_term_term theta) x :=
+  fun n => match n with
+  | S fin_n => (eq_trans) (compSubstSubst_term ((funcomp) (var_term) (shift)) (up_term_term tauterm) ((funcomp) (up_term_term tauterm) (shift)) (fun x => eq_refl) (sigma fin_n)) ((eq_trans) ((eq_sym) (compSubstSubst_term tauterm ((funcomp) (var_term) (shift)) ((funcomp) (subst_term ((funcomp) (var_term ) (shift))) tauterm) (fun x => eq_refl) (sigma fin_n))) ((ap) (subst_term ((funcomp) (var_term ) (shift))) (Eq fin_n)))
+  | 0 => eq_refl
+  end.
+
+Lemma instId_term  : subst_term (var_term ) = (@id) (term ) .
+Proof. exact ((FunctionalExtensionality.functional_extensionality _ _ ) (fun x => idSubst_term (var_term ) (fun n => eq_refl) (((@id) (term )) x))). Qed.
+
+Lemma varL_term   (sigmaterm : (fin)  -> term ) : (funcomp) (subst_term sigmaterm) (var_term ) = sigmaterm .
+Proof. exact ((FunctionalExtensionality.functional_extensionality _ _ ) (fun x => eq_refl)). Qed.
+
+Lemma compComp_term    (sigmaterm : (fin)  -> term ) (tauterm : (fin)  -> term ) (s : term ) : subst_term tauterm (subst_term sigmaterm s) = subst_term ((funcomp) (subst_term tauterm) sigmaterm) s .
+Proof. exact (compSubstSubst_term sigmaterm tauterm (_) (fun n => eq_refl) s). Qed.
+
+Lemma compComp'_term    (sigmaterm : (fin)  -> term ) (tauterm : (fin)  -> term ) : (funcomp) (subst_term tauterm) (subst_term sigmaterm) = subst_term ((funcomp) (subst_term tauterm) sigmaterm) .
+Proof. exact ((FunctionalExtensionality.functional_extensionality _ _ ) (fun n => compComp_term sigmaterm tauterm n)). Qed.
+
+(* **** Forall and Vector.t technology **)
+
+Local Set Implicit Arguments.
+Local Unset Strict Implicit.
+
+Inductive Forall {A : Type} (P : A -> Type) : forall {n}, vector A n -> Type :=
+| Forall_nil : Forall P (@Vector.nil A)
+| Forall_cons : forall n (x : A) (l : vector A n), P x -> Forall P l -> Forall P (@Vector.cons A x n l).
+
+Inductive vec_in {A : Type} (a : A) : forall {n}, vector A n -> Type :=
+| vec_inB {n} (v : vector A n) : vec_in a (cons a v)
+| vec_inS a' {n} (v :vector A n) : vec_in a v -> vec_in a (cons a' v).
+Hint Constructors vec_in.
+
+Lemma strong_term_ind' (p : term -> Type) :
+  (forall x, p (var_term x)) -> (forall F v, (Forall p v) -> p (Func F v)) -> forall (t : term), p t.
+Proof.
+  intros f1 f2. fix strong_term_ind' 1. destruct t as [n|F v].
+  - apply f1.
+  - apply f2. induction v.
+    + econstructor.
+    + econstructor. now eapply strong_term_ind'. eauto.
+Qed.  
+
+Lemma strong_term_ind (p : term -> Type) :
+  (forall x, p (var_term x)) -> (forall F v, (forall t, vec_in t v -> p t) -> p (Func F v)) -> forall (t : term), p t.
+Proof.
+  intros f1 f2. eapply strong_term_ind'.
+  - apply f1.
+  - intros. apply f2. intros t. induction 1; inv X; eauto.
+Qed. 
+
+End fix_sig.
+
+Hint Constructors vec_in.
+  
+
+                                                                     
+
+                                                                     
